<?xml version="1.0" encoding="UTF-8"?>
<section xmlns:xi="http://www.w3.org/2001/XInclude" xml:id="sec_application_set_proofs">
  <title> Application: Set Properties and Equivalences </title>

  <introduction>
    <statement>
      <p>
        This section explores how we can apply the equivalences of logical statements to the set properties we explored in <xref ref="sec_objects_sets"/>. It is no coincidence that those set properties look nearly identical to the logical equivalences!
      </p>
    </statement>
  </introduction>

  <definition>
    <title>Set operations defined via logic</title>
    <statement>
      <p>
        Let <m>A \and B</m> be sets.
        <ol>
          <li>
            <m>A \subseteq B \iff (x \in A) \to (x \in B)</m>
          </li>
          <li>
            <m>x \in A \cup B  \iff x \in A \lor x \in B</m>
          </li>
          
          <li>
            <m>x \in A \cap B  \iff x \in A \land x \in B</m>
          </li>
          
          <li>
            <m>x \in A \setminus B  \iff x \in A \land x \not\in B</m>
          </li>
          <li>
            <m>A = B</m> if and only if <m>A \subseteq B</m> and <m>B \subseteq A</m>.
          </li>
        </ol>
      </p>
    </statement>
  </definition>


  <example>
    <statement>
      <p>
        Prove that if <m>S</m> is any set:
        <ol>
          <li>
            <m>\emptyset \subseteq S</m>
          </li>
          <li>
            <m>S \subseteq S</m>
          </li> 
        </ol>
      </p>
    </statement>
    <solution>
      <p>
        <ol>
          <li>
            <p>
              The logical statement we're trying to prove is <m>(x \in \emptyset) \to (x \in S)</m>
            </p>
            <p>
              Assume that <m>x \in \emptyset</m>. This is false, since nothing is in the empty set. That means that the conditional statement <m>(x \in \emptyset) \to (x\in S)</m> is vacuously true, since the conditional <m>F \to p</m> is always true. Thus <m>\emptyset \subseteq S</m>.
            </p>
          </li>
          <li>
            <p>
              The logical statement we're trying to prove is <m>(x \in S) \to (x\in S)</m>
            </p>
            <p>
              Assume that <m>x \in S</m>. Then <m>x \in S</m> is trivially true. Thus <m>S \subseteq S</m>.
            </p>
          </li>
        </ol>
      </p>
    </solution>
  </example>

  <example>
    <statement>
      <p>
        Prove the following identities:
        <ol>
          <li>
            <m>
              A \cup \emptyset = A
            </m>
          </li>
          <li>
            <m>A \subseteq (A \cup B)</m>
          </li>
          <li>
            <m>A \cap (A \cup B) = A</m>
          </li>
          <li>
            <m>\overline{A \cup B} = \overline{A} \cap \overline{B}</m>
          </li>
        </ol>
      </p>
    </statement>
    <solution>
      <p>
        We'll prove the first via an <q>iff</q> argument:
        <md>
          <mrow> x\in A \cup \emptyset \amp \iff x \in A \lor x\in \emptyset</mrow>
          <mrow> \amp \iff x\in A \lor F</mrow>
          <mrow> \amp \iff x\in A </mrow>
        </md>
        thus <m>A \cup \emptyset = A</m>.
      </p>
    </solution>
  </example>

  <exercises>
    <p>
      Let <m>A, B, \and C</m> be sets. Prove the following identities:
    </p>
    <exercise>
      <statement>
        <p>
          Prove <m>A \cup (B \cup C) = (A \cup B) \cup C</m>
        </p>
      </statement>
      <solution>
        <p>
          Assume <m>x\in A \cup (B \cup C)</m>, then:
          <md>
            <mrow>x\in A \cup (B \cup C) \amp\equiv (x \in A) \lor (x \in B \cup C)</mrow>
            <mrow>\amp\equiv (x \in A) \lor ((x \in B) \lor (x \in C))</mrow>
            <mrow>\amp\equiv x \in A \lor x \in B \lor x \in C</mrow>
            <mrow>\amp\equiv (x \in A \lor x \in B) \lor x \in C</mrow>
            <mrow>\amp\equiv (x \in A \cup B) \lor x \in C</mrow>
            <mrow>\amp\equiv x \in (\in A \cup B) \cup C</mrow>
          </md>
          and so <m>A \cup (B\cup C) = (A \cup B) \cup C</m>.
        </p>
      </solution>
    </exercise>
    <exercise>
      <statement>
        <p>
          Prove <m>\overline{\overline{A}} = A</m>
        </p>
      </statement>
      <solution>
        <p>
          Assume <m>x \in \overline{\overline{A}}</m> then we have
          <md>
            <mrow>x \in \overline{\overline{A}} \amp \equiv \neg(x \in \overline{A})</mrow>
            <mrow>\amp \equiv \neg(\neg (x \in A))</mrow>
            <mrow>\amp \equiv x \in A</mrow>
          </md>
          and so <m>\overline{\overline{A}} = A</m>.
        </p>
      </solution>
    </exercise>
    <!-- <exercise> -->
    <!--   <statement> -->
    <!--     <p> -->
    <!--       Prove <m>A \cup (A \cap B) = A</m> -->
    <!--     </p> -->
    <!--   </statement> -->
    <!--   <solution> -->
    <!--     <p> -->
    <!--       Assume that <m>x \in A \cup (A \cap B)</m>, then: -->
    <!--       <md> -->
    <!--         <mrow>x \in A \cup (A \cap B) \amp \equiv x \in A \lor x\in A \cap B</mrow> -->
    <!--         <mrow>\amp \equiv x \in A \lor (x \in A \land x \in B)</mrow> -->
    <!--         <mrow>\amp \equiv (x \in A \lor x \in A) \land ( x\in A  \lor x \in B )</mrow> -->
    <!--         <mrow>\amp \equiv (x \in A \lor x \in A) \land ( x\in A  ) </mrow> -->
    <!-- I'm getting rid of this one because I need to appeal to simplification which I don't pick up until later. -->
    <!--       </md> -->
    <!--     </p> -->
    <!--   </solution> -->
    <!-- </exercise> -->
    <exercise>
      <statement>
        <p>
          Prove <m>A \cup (B \cap C) = (A \cup B) \cap (A \cup C)</m>
        </p>
      </statement>
      <solution>
        <p>
          <em>Here we convert the expression of sets into a logical statement and apply the distributive law for logical statements.
          </em>
        </p>
        <p>
          Assume that <m>x \in A \cup (B\cap C)</m>, then:
          <md>
            <mrow>x \in A \cup (B \cap C) \amp \equiv x \in A \lor (x \in B \cap C) </mrow>
            <mrow>\amp \equiv x \in A \lor (x\in B \land x \in C)</mrow>
            <mrow>\amp \equiv (x \in A \lor x\in B) \land (x \in A \lor \in C)</mrow>
            <mrow>\amp \equiv (x \in A \cup B) \land (x \in A \cup C)</mrow>
            <mrow>\amp \equiv x \in (A \cup B) \cap (A \cup C)</mrow>
          </md>
          and therefore <m>A \cup (B \cap C) = (A \cup B) \cap (A \cup C)</m>.
        </p>
      </solution>
    </exercise>
    <exercise>
      <statement>
        <p>
          Prove <m>\overline{A \cap B} = \overline{A} \cup \overline{B}</m>
        </p>
      </statement>
      <solution>
        <p>
          <em>Our strategy is to first convert the statement into a logical statement and then apply DeMorgan's law for logical statements.</em>
        </p>
        <p>
          Assume <m>x\in \overline{A \cap B}</m>. Then:
          <md>
            <mrow>\neg (x \in A\cap B) \amp \equiv \neg (x \in A \land x \in B) </mrow>
            <mrow> \amp \equiv \neg (x \in A) \lor \neg (x \in B)</mrow>
            <mrow> \amp \equiv x \in \overline{A} \lor x \in \overline{B}</mrow>
          </md>
          and so <m> \overline{A \cap B} = \overline{A} \cup \overline{B}</m>.
        </p>
      </solution>
    </exercise>
    <exercise>
      <statement>
        <p>
          Prove <m>A \subseteq B</m> if and only if <m>\overline{B} \subseteq \overline{A}</m>
        </p>
      </statement>
      <solution>
        <p>
          <em>Here our <q>trick</q> is to use the fact the the contrapositive is equivalent to the conditional. </em>
        </p>
        <p>
          Assume <m>A \subseteq B</m>. This means that <m>x\in A \to x \in B</m>.
          <md>
            <mrow>x\in A \to x \in B \amp \equiv \neg(x\in B) \to \neg(x \in A) </mrow>
            <mrow> \amp \equiv x \in \overline{B} \to x \in \overline{A}</mrow>
          </md>
          and thus <m>\overline{B} \subseteq \overline{A}</m>.
        </p>
      </solution>
    </exercise>
  </exercises>

 

</section>
