<?xml version="1.0" encoding="UTF-8"?>
<section xmlns:xi="http://www.w3.org/2001/XInclude" xml:id="section-objects-seqseries">
  <title>Sequences and Series</title>

  <definition>
    <p>
      A <term>sequence</term> is a function from a subset of the integers (usually <m>\{0, 1,2,3 \dots\}</m>) to a set <m>S</m>. We use the notation <m>a_n</m> to denote the image of the integer <m>n</m>, and we call <m>a_n</m> the <term><m>n</m>-th term</term> of the sequence.
    </p>
    <p>
      We will often write the shorthand <m>\{a_n\}</m> to denote the complete sequence where <m>n\in \mathbb{N}</m>.
    </p>
  </definition>

  <example>
    <statement>
      <p>
        Find <m>a_1, a_2, a_3, a_4</m> for the sequences:
      </p>
      <ol>
        <li><m>a_n = \frac{1}{n^2}</m></li>
        <li><m>a_n = 3\cdot 2^n</m></li>
        <li><m>a_n = -5 + 3n</m></li>
      </ol>
    </statement>
    <answer>
      <video youtube="ZNgKw-fIzLk"/>
    </answer>

  </example>

  <definition>
    <p>
      A <term>geometric progression</term> is a sequence of the form:
      <me>a, ar, ar^2, ar^3, \dots, ar^n, \dots </me>
      with the <term>initial term</term> <m>a</m> and the <term>common ratio</term> <m>r</m>.
    </p>
    <p>
      A <term>arithmetic progression</term> is a sequence of the form:
      <me>a, a+d, a+2d, a+3d, \dots, a+nd, \dots </me>
      with the <term>initial term</term> <m>a</m> and the <term>common difference</term> <m>d</m>.
    </p>
  </definition>

  <definition>
    <p>
      A <term>recurrence relation</term> for a sequence <m>\{a_n\}</m> is an equation that expressions <m>a_n</m> in terms of previous terms.
    </p>
    <p>
      A sequence is called a <term>solution</term> of a recurrence relation if its terms satisfy the recurrence relation.
    </p>
    <p>
      We can always think of a sequence as a function, so the recurrence <m>a_n = a_{n-1} + a_{n-2}</m> is the function:
      <cd>
        def a(n):
            return a(n-1) + a(n-1)
      </cd>
      with infinite recursion.
    </p>
  </definition>

  <example xml:id="fib-def">
    <statement>
      <p>
        The <term>Fibonacci sequence</term> <m>F_0, F_1, F_2, \dots</m> is defined by the recurrence:
        <me>F_n = F_{n-1} + F_{n-2} \text{ For } n \ge 2, \text{ where } F_0 = 0, F_1 = 1 </me>
      </p>
      <p>
        Note that the Fibonacci sequence has both the recursive definition <em>and</em> a definition for the first two terms of the sequence.
      </p>
    </statement>
    <answer>
      <video youtube="zo_GYIP61i8"/>
    </answer>

  </example>

  <example>
    <statement>
      <p>
        Consider the recurrence <m>a_n = -3 a_{n-1} + 4 a_{n-2}</m>. Are the following sequences solutions to the recurrence?
      </p>
      <ol cols="2">
        <li><m>a_n = 0</m></li>
        <li><m>a_n = 1</m></li>
        <li><m>a_n = 2^n</m></li>
        <li><m>a_n = (-4)^n</m></li>
      </ol>
    </statement>
    <answer>
      <video youtube="4HTdTrMp9sY"/>
    </answer>

  </example>

  <note>
    <p>
      A recurrence has a unique solution if it has initial data.
    </p>
    <p>
      This would be a function defined with finite recursion, so the recurrence <m>F_n = F_{n-1} + F_{n-2}</m> with <m>F_0 = 0</m> and <m>F_1=1</m>, the Fibonacci sequence, is the function:
      <cd>
        def F(n):
            if n == 0:
                return 0
            elif n == 1:
                return 1
            else:
                return F(n-1) + F(n-1)
      </cd>
    </p>
  </note>

  <example>
    <statement>
      <p>
        Find the unique solution to each recurrence:
      </p>
      <ol>
        <li><m>a_n = 2a_{n-1} - 3</m> with <m>a_0 = -1</m></li>
        <li><m>a_n = 2n a_{n-1}</m> with <m>a_0 = 3</m></li>
      </ol>
    </statement>
    <answer>
      <video youtube="e3bMOe2fbKg"/>
      <video youtube="gBSNZsWxRZ8"/>
    </answer>

  </example>

  <note>
    <p>
      When finding the general form of a sequence, creativity is required.
    </p>
    <p>
      Look for patterns within the sequence
      <ul>
        <li>Look for a common difference (arithmetic)</li>
        <li>Look for a common ratio (geometric)</li>
        <li>Do later terms depend on previous terms in a recursive way?</li>
        <li>Are there cycles among the terms?</li>
        <li>...</li>
      </ul>
    </p>
  </note>


  <example>
    <statement>
      <p>
        Find a simple formula or rule that generates the terms of the sequence, and give the next three terms of the sequence.
      </p>
      <ol>
        <li><m>7, 11, 15, 19, 23, 27, 31, \dots</m></li>
        <li><m>1, 10, 11, 100, 101, 110, 111, 1000, \dots</m></li>
        <li><m>1, 3, 15, 105, 945, 10395, 135135, \dots</m></li>
        <li><m>2,2,2,3,3,3,3,3, 5,5,5,5,5,5,5,\dots</m></li>
        <li><m>2,4,16,256,65536, 4294957296, \dots</m></li>
      </ol>
      
      <p>
        For this last example, the numbers are huge. If you're reading on the web-based version of this book, this is an interactive calulator. You can type what you want to compute and press 'Evaluate (Sage).' For more information, refer to the <xref ref="appendix_sage_howto">Sage appendix</xref>
      </p>
      <sage>
        <input>
          16^2
        </input>
        <output>
          256
        </output>
      </sage>
    </statement>
  </example>

  <definition>
    <p>
      Let <m>\{a_n\}</m> be a sequence. We define a <term>series</term> of the sequence to be the summation of some subset of the terms of the sequence. We denote the sum by a capital sigma with sub- and superscript information in the following conventional way:
      <me>\sum_{\text{index variable, lower bound}}^{\text{upper bound}} \text{(sequence rule in terms of index variable)}</me>
    </p>
    <p>
      For example, the summation of terms from 0 to <m>n</m> is expressed:
      <me>\sum_{i=0}^n a_i = a_0 + a_1 + a_2 + \dots + a_{n-1} + a_n</me>
    </p>
  </definition>

  <example>
    <statement>
      <p>
        Find the value of the sum:
      </p>
      <ol cols="2">
        <li><m>\displaystyle \sum_{j=0}^8 (1 + (-1)^j)</m></li>
        <li><m>\displaystyle \sum_{k \in \{1, 3, 5\}} (k^2 + 2)</m></li>
        <li><m>\displaystyle \sum_{j=1}^2 \sum_{k=1}^5 (j-k) </m></li>
        <li><m>\displaystyle \sum_{j=1}^2 \sum_{k=1}^5 (k-j) </m></li>
      </ol>
    </statement>
    <answer>
      <video youtube="dCVopWx51sc"/>
    </answer>

  </example>

  <example xml:id="example-geometric-series">
    <statement>
      <p>
        Verify the following formula for the sum of a geometric sequence, if <m>r \not= 1</m>,
        <me>\sum_{k=0}^n ar^k = \frac{a-ar^{n+1}}{1-r}</me>.
      </p>
    </statement>
    <answer>
      <video youtube="K8eg6Cd_QL8"/>
    </answer>

  </example>


  <example xml:id="example-telescoping-sum">
    <statement>
      <p>
        Show that <me>\sum_{j=1}^n (a_j - a_{j-1}) = a_n - a_0</me>
      </p>
    </statement>
    <answer>
      <video youtube="xY9ZHorCv4I"/>
    </answer>

  </example>

  <example xml:id="example-sum-of-integers">
    <statement>
      <p>
        Find a formula for the following sums, using the <xref ref="example-telescoping-sum">telescoping example</xref>:
      </p>
      <ol>
        <!-- <li><m>\displaystyle \sum_{k=1}^n (2k -1) </m>, the sum of the first <m>n</m> odd numbers.</li> -->
        <li>Using the sequence <m>a_n=n^2</m>, find a formula for the sum <m>\displaystyle \sum_{k=1}^n k</m> by the finding the sum two ways.</li>
      </ol>
    </statement>
    <answer>
      <video youtube="1SD1LJv22Cg"/>
    </answer>

  </example>

  <note xml:id="note-some-sum-formulas">
    <statement>
      <p>
        <xref ref="example-sum-of-integers"/> shows us the following formula for an arithmetic series:
        <me> \displaystyle \sum_{k=1}^n k = \dfrac{n(n+1)}{2}</me>
      </p>
      <p>
        We will verify in <xref ref="exercise-sum-of-squares"/> sum formula for the series of squares:
        <me> \displaystyle \sum_{k=1}^n k^2 = \dfrac{n(2n+1)(n+1)}{6}</me>
      </p>
    </statement>
  </note>

  <assemblage>
    <title>Computer Corner</title>
    <caption>Computer Corner</caption>
    <p>
      Recurrence relations are like recursive functions. For example, you can find the <m>n</m>th Fibonacci number, <m>F_n</m>, by evaluating <c>fibonacci(n)</c>
      <sage language="python">
        <input>
def fibonacci(n):
    if n == 0:
        return 0
    elif n== 1:
        return 1
    return fibonacci(n-1) + fibonacci(n-2)

## list out the first 21 fibonacci numbers
print(list(map(fibonacci, range(0, 20))))

## Just type fibonacci(15) to get the 15th fibonacci number.
        </input>
      </sage>
    </p>
    <p>
      The initial conditions of a a recurrence guarantee that it has a unique solution. These initial conditions are the terminal/base conditions for the recursive functions. Because it's theoretical, math can go on forever, computers enter infinite loops:
      <sage language="python">
        <input>
def forever(n):
    # no base case; won't stop
    return forever(n-1)

forever(1)
## press Evaluate(Python) to watch it go on forever. The algorithm won't halt until the runtime stack runs out of memory.
        </input>
      </sage>
      Eventually, we'll get <c>RecursionError: maximum recursion depth exceeded while calling a Python object</c>
    </p>
  </assemblage>

  <exercises>
    <exercise>
      <statement>
        <p>
          Find the first five terms of the sequence <m>\{a_n\}</m>, beginning with <m>n=0</m>:
        </p>
        <ol cols="2">
          <li><m>a_n = 2^n + 3</m></li>
          <li><m>a_n = n^{n+1}</m></li>
          <li><m>a_n = \lfloor n/2\rfloor + \lceil n/2 \rceil</m></li>
          <li><m>a_n = 6a_{n-1},\hspace{1em} a_0 = 2</m></li>
          <li><m>a_n = a_{n-1} + 3 a_{n-2},\hspace{1em} {a_0 = 1, a_1 = 2}</m></li>
        </ol>
      </statement>
      <solution>
        <p>
          <ol>
            <li><m>\{4, 5, 7, 11, 19\}</m></li>
            <li><m>\{ 0, 1, 8, 81, 1024 \}</m></li>
            <li><m>\{ 0, 1, 2, 3, 4\}</m></li>
            <li><m>\{2, 12, 72, 432, 2592 \}</m></li>
            <li><m>\{1, 2, 5, 11, 26\}</m></li>
          </ol>
        </p>
      </solution>

    </exercise>

    <exercise>
      <statement>
        <p>
          Is the sequence <m>\{a_n\}</m> a solution of the recurrence relation <m>{a_n = 8a_{n-1}-16a_{n-2}}</m> if
          <ol cols="2">
            <li><m>a_n = 0</m></li>
            <li><m>a_n = 2n</m></li>
            <li><m>a_n = 2^n</m> </li>
            <li><m>a_n = 4^n</m> </li>
          </ol>
        </p>
      </statement>
      <solution>
        <p>
          <ol>
            <li>Yes</li>
            <li>No</li>
            <li>No</li>
            <li>Yes</li>
          </ol>
        </p>
      </solution>

    </exercise>

    <exercise>
      <statement>
        <p>
          Find a solution to the recurrence relation
          <ol>
            <li><m>a_n = 3a_{n-1},\hspace{1em} a_0 = 2</m></li>
            <li><m>a_n = a_{n-1} + n,\hspace{1em} a_0 = 1</m></li>
            <li><m>a_n = na_{n-1},\hspace{1em} a_0 = 1</m></li>
          </ol>
        </p>
      </statement>
      <solution>
        <p>
          <ol>
            <li><m>a_n = 2\cdot 3^n</m></li>
            <li><m>a_n = \dfrac{n^2 + n + 2}{2}</m></li>
            <li><m>a_n = n!</m></li>
          </ol>

        </p>
      </solution>

    </exercise>

    <exercise>
      <statement>
        <p>
          Find the value of each of the following sums:
          <ol cols="2">
            <li> <m>\displaystyle \sum_{k=0}^8 3\cdot 2^k</m> </li>
            <li> <m>\displaystyle \sum_{k=1}^8 2^k </m> </li>
            <li> <m>\displaystyle \sum_{k=1}^8 (1 + (-1)^k) </m> </li>
            <li> <m>\displaystyle \sum_{k=1}^8 (2^{k+1} - 2^k) </m> </li>
            <li><m>\displaystyle \sum_{k=50}^{100} k</m></li>
          </ol>
        </p>
      </statement>
      <solution>
        <p>
          <ol>
            <li> 1533</li>
            <li> 510 </li>
            <li> 8 </li>
            <li> 510 </li>
            <li> 3825 </li>
          </ol>
        </p>
      </solution>

    </exercise>

    <exercise xml:id="exercise-sum-of-squares">
      <statement>
        <p>
          Using <xref ref="example-telescoping-sum">the telescoping example</xref> with the sequence <m>a_n=(n+1)^3</m>, derive a formula for <m>\displaystyle \sum_{k=1}^n k^2</m>
        </p>
      </statement>
      <solution>
      <p>
        This one's a lot of fun, so let's do it in a lot of detail. This is approach Blaise Pascal used to discover the formula in his 1654 <pubtitle>Traité du triangle arithmétique</pubtitle>.
      </p>
      <p>
        Let <m>a_n = (n+1)^3</m>. Then from <xref ref="example-telescoping-sum">example</xref>, we have that:
        <md>
          <mrow>\sum_{j=1}^n (j+1)^3 - j^3 &amp; = a_n - a_0</mrow>
          <mrow>\sum_{j=1}^n (j+1)^3 - j^3 &amp; = (n+1)^3 - (0+1)^3</mrow>
          <mrow>\sum_{j=1}^n j^3 + 3j^2 + 3j + 1 - j^3 &amp; = n^3 + 3n^2 + 3n + 1 - 1</mrow>
          <mrow>\sum_{j=1}^n 3j^2 + 3j + 1 &amp; = n^3 + 3n^2 + 3n </mrow>
          <mrow>\sum_{j=1}^n 3j^2 + \sum_{j=1}^n 3j + \sum_{j=1}^n 1 &amp; = n^3 + 3n^2 + 3n </mrow>
          <mrow> 3 \sum_{j=1}^n j^2 + 3 \sum_{j=1}^n j + \sum_{j=1}^n 1 &amp; = n^3 + 3n^2 + 3n </mrow>
          <mrow> 3 \sum_{j=1}^n j^2 &amp; = n^3 + 3n^2 + 3n - 3 \sum_{j=1}^n j - \sum_{j=1}^n 1 </mrow>
          </md>

          </p>
          <p> We have from <xref ref="example-sum-of-integers">example</xref> that <m>\displaystyle \sum_{j=1}^n j = \dfrac{n(n+1)}{2}</m> and if we add <m>1</m> a total of <m>n</m> times, we have <m>\displaystyle \sum_{j=1}^n 1 = n</m>. Plugging these in, we find:
          </p>
          <p>
            <md>
          <mrow> 3 \sum_{j=1}^n j^2  &amp; = n^3 + 3n^2 + 3n - 3 \sum_{j=1}^n j - \sum_{j=1}^n 1 </mrow>
          <mrow> 3 \sum_{j=1}^n j^2  &amp; = n^3 + 3n^2 + 3n - 3\left( \dfrac{n(n+1)}{2}\right) - n</mrow>
          <mrow> 3 \sum_{j=1}^n j^2  &amp; = n^3 + 3n^2 + 2n - 3\left(\dfrac{n^2 + n}{2}\right) </mrow>
          <mrow> 3 \sum_{j=1}^n j^2  &amp; = \frac{2n^3}{2} + \frac{6n^2}{2} + \frac{4n}{2} - \dfrac{3n^2}{2} - \frac{3n}{2}</mrow>
          <mrow> 3 \sum_{j=1}^n j^2  &amp; = \frac{2n^3 + 3n^2 + n}{2}  </mrow>
          <mrow> 3 \sum_{j=1}^n j^2  &amp; = \frac{n(2n+1)(n+1)}{2}  </mrow>
          <mrow> \sum_{j=1}^n j^2  &amp; = \frac{n(2n+1)(n+1)}{6}  </mrow>
          </md>

          which is exactly the formula you learned in calculus!
          </p>
      </solution>
    </exercise>

    <exercise>
    <statement>
      <p>
        Use <xref ref="example-geometric-series">the formula for geometric series</xref> to show that
        <me>1 + 2 + 2^2 + 2^3 + \dots 2^n = 2^{n+1} - 1</me>
      </p>
    </statement>
    <solution>
      <p>
        Noting that this is a geometric series with common ratio 2 and first term 1, let <m>r=2, a=1</m> in the geometric series formula:

        <md>
          <mrow>\sum_{k=0}^n 2^{k} \amp= \dfrac{1-2^{n+1}}{1-2}</mrow>
          <mrow> \amp= 2^{n+1} - 1</mrow>
        </md>

        This is why a binary number which is all 1's is always one less than the next power of 2, e.g. <m>1111_{\text{two}} = 15_{\text{ten}}</m>
      </p>
    </solution>
    </exercise>
  </exercises>

  <subsection>
    <title>Forum Posts about this section</title>

    <slate xml:id="discourse" surface="html" >
      <div id='discourse-comments'></div>
      <script type="text/javascript">
        DiscourseEmbed = { discourseUrl: 'https://discourse.math.wichita.edu/',
        topicId: 298 };

        (function() {
        var d = document.createElement('script'); d.type = 'text/javascript'; d.async = true;
        d.src = DiscourseEmbed.discourseUrl + 'javascripts/embed.js';
        (document.getElementsByTagName('head')[0] || document.getElementsByTagName('body')[0]).appendChild(d);
        })();
      </script>
    </slate>
  </subsection>

</section>
