<?xml version="1.0" encoding="UTF-8"?>
<section xmlns:xi="http://www.w3.org/2001/XInclude" xml:id="section-logic-arguments">
  <title>Logical Arguments</title>

  <definition>
    <p>
      An <term>argument</term> is a sequence of statements (<term>premises</term>) that ends with a conclusion.
    </p>
    <p>
      A <term>valid argument</term> is one where the conclusion follows from the truth of the premises.
    </p>
    <p>
      For the sequence of premises <m>p_1, p_2, \dots, p_n</m> and conclusion <m>q</m>, an argument is valid if:
      <me>p_1 \wedge p_2 \wedge \dots \wedge p_n \to q</me> is a tautology.
    </p>
    <p>
      A <term>fallacy</term> is a form of incorrect reasoning that leads to an invalid argument.
    </p>
  </definition>

  <example>
    <statement>
      <p>
        Consider the following argument:
        <ul>
          <li>If you give a mouse a cookie, then he'll ask for a glass of milk.</li>
          <li>You gave a mouse a cookie.</li>
          <li>Therefore he asked for a glass of milk.</li>
        </ul>
      </p>
      <p>
        This argument is of the form:
        <tabular halign="right">
          <row>
            <cell><m>p \to q</m></cell>
          </row>
          <row bottom="minor">
            <cell><m> p</m></cell>
          </row>
          <row>
            <cell><m>\therefore q</m></cell>
          </row>
        </tabular>
        and is valid since <m> ((p \to q) \wedge p) \to q</m> is a tautology.
      </p>
    </statement>
  </example>

  <p> Below is a table of common argument forms, also known as rules of inference. Observe that we're using <m>\Rightarrow</m> to show <q>if, then</q>. This symbolic choice is to highlight the difference between the hypotheses and conclusion of the argument, and carries no additional meaning for the purposes of this course.</p>

  <list xml:id="list-logical-arguments">
    <title>
      Basic argument forms - rule of inference
    </title>

    <introduction>
      Let <m>p, q \and r</m> be logical propositions. The following are tautologies:
    </introduction>

    <dl width="narrow">
      <li>
        <title>Modus Ponens/Direct reasoning</title>
        <p>
          <m>(p\to q) \land p \Rightarrow q</m>
        </p>
      </li>
      <li>
        <title>Modus Tollens / Indirect Reasoning</title>
        <p>
          <m>(p \to  q) \land  \neg q \Rightarrow  \neg p</m>
        </p>
      </li>
      <li>
        <title>Disjunctive Addition</title>
        <p>
          <m>p\Rightarrow (p\lor q)</m>
        </p>
      </li>
      <li>
        <title>Conjunctive Simplification</title>
        <p>
          <m>(p \land  q) \Rightarrow  p</m>
          <line/> <line/>
          <m>(p \land  q) \Rightarrow  q</m>
        </p>
      </li>
      <li>
        <title>Disjunctive Simplification</title>
        <p>
          <m>(p \lor  q) \land  \neg p \Rightarrow  q</m>
          <line/>
          <m>(p \lor q) \land \neg q\Rightarrow p</m>
        </p>
      </li>
      <li>
        <title>Chain Argument / Syllogism</title>
        <p>
          <m>(p \to  q) \land  ( q \rightarrow  r) \Rightarrow  (p\to  r)</m>
        </p>
      </li>
      <li>
        <title>Biconditional Equivalences</title>
        <p>
          <m>(p \leftrightarrow  q) \equiv  (p\rightarrow q) \land  (q \rightarrow  p)</m><line/>
          <m>(p \leftrightarrow  q) \equiv (p \land  q) \lor  (\neg p \land  \neg q)</m>
        </p>
      </li>
      <li>
        <title>Implication / Conditional Equivalence</title>
        <p>
          <m>p \rightarrow  q \equiv  \neg p \lor  q</m>
        </p>
      </li>
      <li>
        <title>Contraposition</title>
        <p>
          <m>(p\to q) \equiv (\neg q \to \neg p)</m>
        </p>
      </li>
    </dl>
  </list>

  <note>
    <statement>
      <p>
        It would be good practice to verify that each of the arguments in table <xref ref="list-logical-arguments"/> is a tautology using either true tables or logical equivalences.
      </p>
    </statement>
  </note>

  <example>
    <statement>
      <p>
        What rules of inference are being used here?
      </p>
      <ul>
        <li>Kangaroos live in Australia and are marsupials. Therefore, kangaroos are marsupials. </li>
        <li> If I go swimming, then I will stay in the sun too long. If I stay in the sun too long, then I will sunburn. Therefore, if I go swimming, then I will sunburn. </li>
        <li>I read a horror story. When I read horror stories, I have weird dreams. Therefore I had weird dreams.</li>
      </ul>
    </statement>
  </example>

  <definition>
    <p>
      <term>Existential instantiation</term> describes the argument:
      <me> \exists x P(x) \implies P(c) </me> for some <m>c</m> in the domain.
    </p>
    <p>
      <term>Existential generalization</term> describes the argument:
      <me> P(c) \implies \exists x P(x) </me>.
    </p>
    <p>
      <term>Universal modus ponens</term> describes the argument:
      <me>\forall x (P(x) \to Q(x)) \wedge P(a) \implies Q(a)</me> where <m>a</m> is a particular element in the domain.
    </p>
    <p>
      <term>Universal modus tollens</term> describes the argument:
      <me>\forall x (P(x) \to Q(x)) \wedge \neg Q(a) \implies \neg P(a)</me> where <m>a</m> is a particular element in the domain.
    </p>
    
  </definition>

  <example>
    <statement>
      <p>
        Show that the premises, <q>A student in this class has not read the book,</q> and <q>Everyone in this class passed the first exam</q> imply the conclusion <q>Someone who passed the first exam has not read the book.</q> Let <m>C(x)</m> be <q><m>x</m> is in this class,</q> <m>B(x)</m> <q>x has read the book</q>, and <m>P(x)</m> <q><m>x</m> passed the first exam.</q>
      </p>
    </statement>
    <solution>
      <p> The statement, <q>someone who passed the first exam has not read the book</q> means there is someone in class did those things. <m>\exists x (P(x) \wedge \neg B(x))</m></p>
      <table>
        <title>Argument step-by-step</title>
        <tabular>
          <col />
          <col />
          <row bottom="minor" header="yes">
            <cell> Step</cell> 
            <cell> Reason </cell>
          </row>
          <row>
            <cell> 1. <m>\exists x(C(x) \wedge \neg B(x))</m> </cell>
            <cell> Premise </cell>
          </row>
          <row>
            <cell> 2. <m>C(a) \wedge \neg B(a) </m> </cell>
            <cell> Existential instantiation  </cell>
          </row>
          <row>
            <cell> 3. <m>C(a)</m> </cell>
            <cell> Simplification of 2</cell>
          </row>
          <row>
            <cell> 4. <m>\forall x (C(x) \to P(x))</m> </cell>
            <cell> Premise </cell>
          </row>
          <row>
            <cell> 5. <m>C(a) \to P(a)</m> </cell>
            <cell> Universal instantiation </cell>
          </row>
          <row>
            <cell> 6. <m>P(a)</m> </cell>
            <cell> Modus ponens of 3 and 5 </cell>
          </row>
          <row>
            <cell> 7. <m>\neg B(a)</m> </cell>
            <cell> simplification of 2 a different way</cell>
          </row>
          <row>
            <cell> 8. <m>P(a) \wedge \neg B(a)</m> </cell>
            <cell> Conjunction of 6 and 7</cell>
          </row>
          <row>
            <cell> 9 . <m>\exists x (P(x) \wedge \neg B(x))</m> </cell>
            <cell> Existential generalization from 8.</cell>
          </row>
        </tabular>
      </table>
    </solution>
  </example>

  <example>
    <statement>
      <p>
        For the following argument, explain the rules of inference for each step leading the the conclusion:
      </p>
      <p>
        <blockquote>
          <p>Linda, a student in this class owns a red convertible. Everyone who owns a red convertible has gotten at least one speeding ticket. Therefore, someone in this class has gotten at least one speeding ticket.
          </p>
        </blockquote>
      </p>
    </statement>
    <!--
        Let $C(X)$ be the statement ``$x$ is in this class.'' 
    
    Let $R(X)$ be the statement ``$x$ has a red convertible.''
    
    Let $S(X)$ be the statement ``$x$ has gotten at least one speeding ticket.''
    
    \hspace{1em}
    
    \begin{tabular}{l|l}  % a fill in the blank table 
         Step & Reason  \\
         \hline 
         1. $C(\mbox{Linda}) \land R(\mbox{Linda})$& \\
         2. $R(\mbox{Linda})$ & \\
         3. $\forall x (R(x) \to S(x)$  & \\ 
         4. $R(\mbox{Linda}) \to S(\mbox{Linda})$ & \\
         5. $S(\mbox{Linda})$ & \\
         6. $C(\mbox{Linda}) \land S(\mbox{Linda})$ & \\
         7. $\exists x (C(x) \land S(x)) $ & \\
    \end{tabular}  
        //-->
  </example>

  <p>
    Here are some common fallacies. They're not typeset in a table because although you should be aware of what they are, they are not valid arguments!
    <ul>
      <li>
        <p>Fallacy of affirming the conclusion:
        <ul>
          <li><q>If you get an A, you pass this class. You passed the class, therefore you got an A.</q>   (not valid!)
          </li>
          <li><q>If an animal is a type of cat, it has hair. I have hair. Therefore, I must be some kind of cat.</q> (not valid!) </li>
          <li> <m> ((p \to q) \wedge q \to p)</m> is not a tautology! </li>
        </ul>
        </p>
      </li>
      <li>
        <p>
          Fallacy of denying the hypothesis
          <ul>
            <li><q>If you get an A, you pass this class. You didn't get an A. Oh no! You must not have passed this class!</q> (still not valid!)</li>
            <li><q>If an animal is a type of cat, it has hair. My dog Ruby isn't a cat. Therefore she must not have hair.</q> (nope) </li>
            <li> <m> ((p\to q) \wedge \neg p \to q)</m> is not a tautology!</li>
          </ul>
        </p>
      </li>
    </ul>
  </p>


  <exercises>


    <!-- the following comes from https://github.com/oscarlevin/discrete-book -->
    <exercise>
      <statement>
        <p>
          Determine if the following deduction rule is valid:
        </p>
        <tabular halign="right">
          <row>
            <cell><m>p \vee q</m></cell>
          </row>
          <row bottom="minor">
            <cell><m>\neg p</m></cell>
          </row>
          <row>
            <cell><m>\therefore q</m></cell>
          </row>
        </tabular>
      </statement>
      <solution>
        <p>
          The deduction rule is valid. To see this, make a truth table which contains <m>p \vee q</m> and <m>\neg p</m> (and <m>p</m> and <m>q</m> of course). Look at the truth value of <m>q</m> in each of the rows that have <m>p \vee q</m> and <m>\neg p</m> true.
        </p>
      </solution>
    </exercise>

    <!-- the following is adapted from https://github.com/oscarlevin/discrete-book -->
    <exercise>
      <statement>
        <p>
          Determine if the following is a valid deduction rule:
        </p>
        <tabular halign="right">
          <row>
            <cell><m>p \to (q \vee r)</m></cell>
          </row>
          <row bottom="minor">
            <cell><m>\neg(p \to q)</m></cell>
          </row>
          <row>
            <cell><m>\therefore r</m></cell>
          </row>
        </tabular>
      </statement>
      <solution>
        <p>
          This is valid. Make a truth table.
        </p>
      </solution>

    </exercise>

    <!-- the following is adapted from https://github.com/oscarlevin/discrete-book -->
    <exercise>
      <statement>
        <p>
          Determine if the following is a valid deduction rule:
        </p>
        <tabular halign="right">
          <row>
            <cell><m>(p \wedge q) \to r</m></cell>
          </row>
          <row bottom="minor">
            <cell><m>\neg p \vee \neg q</m></cell>
          </row>
          <row>
            <cell><m>\therefore \neg r</m></cell>
          </row>
        </tabular>
      </statement>
      <solution>
        <p>
          It isn't; make a truth table and see <m>(((p \land q) \to r) \land (\neg p \lor \neg q)) \to \neg r</m> isn't a tautology.
        </p>
      </solution>
    </exercise>



    <exercise>
      <statement>
        <p>
          Show that the following is a valid deduction rule by building a truth table.
        </p>
        <p>
          <tabular halign="right">
            <row>
              <cell><m>p \to q</m></cell>
            </row>
            <row bottom="minor">
              <cell><m>q \to r</m></cell>
            </row>
            <row>
              <cell><m>\therefore (p \to r)</m></cell>
            </row>
          </tabular>
        </p>
      </statement>
      <!-- <solution> -->
      <!--   <p> -->
      <!--     <em>First, write the argument as the logical statement and simplify using equivalences. As usual, any time we have conditional statements, we use implication to turn them into disjunctions.</em> -->
      <!--     <md> -->
      <!--       <mrow>((p \to q) \land (q \to r)) \to (p \to r) \amp \equiv \neg((\neg p \lor q) \land (\neg q \lor r)) \lor (\neg p \lor r)</mrow> -->
      <!--       <mrow>\amp \equiv \neg(\neg p \lor q) \lor \neg (\neg q \lor r) \lor (\neg p \lor r)</mrow> -->
      <!--       <mrow>\amp \equiv (p \land \neg q) \lor (q \land \neg r) \lor (\neg p \lor r)</mrow> -->
      <!--       <mrow> \text{ then distributive... this is a mess for intro class maybe } </mrow> -->
      <!--     </md> -->
      <!--   </p> -->
      <!-- </solution> -->
    </exercise>

    <exercise>
      <statement>
        <p>
          Come up with all valid conclusions for this set of premises: <q>If you get out the leash, the dog wants to go for a walk,</q> <q>the dog wants to go for a  walk if you put on shoes,</q> <q>the dog wanting to go for a walk is sufficient for me to want a cat.</q> <q>The dog doesn't want to go for a walk.</q> Explain your answer noting each step of the argument.
        </p>
      </statement>
    </exercise>

    <exercise>
      <statement>
        <p>
          Consider the statement <q>Superman saves the day or Lois Lane dies. Superman saved the day, therefore Lois didn't die.</q> Is the argument valid? Explain your answer.
        </p>
      </statement>
      <solution>
        <p>
          This is an argument of the form:
          <tabular halign="right">
            <row>
              <cell><m>\text{Superman saves} \lor \text{Lois dies}</m></cell>
            </row>
            <row bottom="minor">
              <cell><m>\text{Superman saved}</m></cell>
            </row>
            <row>
              <cell><m>\therefore \neg \text{Lois didn't die}</m></cell>
            </row>
          </tabular>
          This is a fallacy. In fact, it's the fallacy of denying the hypothesis in disguise. Rewrite the disjunction as an implication to see this:
          <tabular halign="right">
            <row>
              <cell><m>\neg \text{Superman saves} \to \text{Lois dies}</m></cell>
            </row>
            <row bottom="minor">
              <cell><m>\text{Superman saved}</m></cell>
            </row>
            <row>
              <cell><m>\therefore \neg \text{Lois didn't die}</m></cell>
            </row>
          </tabular>
        </p>
      </solution>
    </exercise>


    <exercise>
      <statement>
        <p>
          Prove that the folowing is a valid argument, explaining each rule of inference used to arrive at the conclusion.
          <ol>
            <li>
              <p>
                <q>I take the bus or I walk. If I walk I get tired. I do not get tired. Therefore I take the bus. </q>
              </p>
            </li>
            <li>
              <p>
                <q>All lions are fierce. Some lions do not drink coffee. Therefore, some fierce creatures do not drink coffee.</q>
              </p>
            </li>
          </ol>
        </p>
      </statement>
      <hint>
        <p>
          <ol>
            <li>Write each in terms of logical symbols.</li>
            <li>Let the universe of discourse be all creatures, <m>L(x)</m> be the statement <q><m>x</m> is a lion,</q> <m>C(x)</m> be <q><m>x</m> drinks coffee,</q> and <m>F(x)</m> is <q><m>x</m> is fierce.</q></li>
          </ol>
        </p>
      </hint>
    </exercise>

    <!-- This exercise is adapted from Al Doerr, Ken Levasseur, Applied Discrete Structures -->
    <exercise>
      <statement>
        <p>
          Show that the following argument is invalid.
        </p>
        <p>
          If wages increase, then there will be inflation. The cost of living will not increase if there is no inflation. Wages will increase. Therefore, the cost of living will increase.
        </p>
      </statement>
      <hint>
        <p>
          Make a truth table.
        </p>
      </hint>
      <solution>
        <p>
          The argument has three propositional variables and is of the form:
          <tabular halign="right">
            <row>
              <cell><m>\text{wages increase} \to \text{inflation}</m></cell>
            </row>
            <row>
              <cell><m>\neg\text{inflation} \to \neg \text{cost of living increase}</m></cell>
            </row>
            <row bottom="minor">
              <cell><m>\text{wages increase}</m></cell>
            </row>
            <row>
              <cell><m>\therefore \text{cost of living increases}</m></cell>
            </row>
          </tabular>
          ... now make a truth table.
        </p>
      </solution>
    </exercise>

  </exercises>

</section>
